Clean/Gadgets/Keccak/ThetaD.lean
@@ -45,7 +45,7 @@ theorem soundness : Soundness (F p) elaborated Assumptions Spec := by
   simp only [zero_sub, Fin.coe_neg_one, and_imp, add_assoc, Nat.reduceAdd] at h_holds
   simp only [circuit_norm, KeccakRow.normalized_iff, KeccakRow.value, eval_vector]
 
-  have s (i : ℕ) (hi : i < 5) : ProvableType.eval' env (row_var[i]) = row[i] := by
+  have s (i : ℕ) (hi : i < 5) : eval env (row_var[i]) = row[i] := by
     rw [←h_input, Vector.getElem_map]
 
   simp only [s] at h_holds
@@ -74,9 +74,8 @@ theorem soundness : Soundness (F p) elaborated Assumptions Spec := by
   simp [Specs.Keccak256.thetaD, h_xor0, h_xor1, h_xor2, h_xor3, h_xor4, rotLeft64]
 
 theorem completeness : Completeness (F p) elaborated Assumptions := by
-  intro i0 env row_var h_env row h_input h_assumptions
-  simp only [Assumptions, KeccakRow.normalized_iff] at h_assumptions
-  dsimp only [circuit_norm, main, Xor64.circuit, Rotation64.circuit, Rotation64.elaborated] at h_env ⊢
+  circuit_proof_start [Xor64.circuit, Rotation64.circuit, Rotation64.elaborated]
+  simp only [KeccakRow.normalized_iff] at h_assumptions
   simp_all only [circuit_norm, getElem_eval_vector,
     Xor64.Assumptions, Xor64.Spec, Rotation64.Assumptions, Rotation64.Spec,
     add_assoc, seval, true_and]
